% Created 2023-05-22 lun 17:27
% Intended LaTeX compiler: pdflatex
\documentclass[11pt]{article}
\usepackage[utf8]{inputenc}
\usepackage[T1]{fontenc}
\usepackage{graphicx}
\usepackage{longtable}
\usepackage{wrapfig}
\usepackage{rotating}
\usepackage[normalem]{ulem}
\usepackage{amsmath}
\usepackage{amssymb}
\usepackage{capt-of}
\usepackage{hyperref}
\author{Diego Vila}
\date{\textit{[2022-12-23 vie 02:01]}}
\title{exponents}
\hypersetup{
 pdfauthor={Diego Vila},
 pdftitle={exponents},
 pdfkeywords={},
 pdfsubject={},
 pdfcreator={Emacs 28.2 (Org mode 9.7-pre)}, 
 pdflang={English}}
\begin{document}

\maketitle
\tableofcontents

\(2^5 = 5 \times 5 \times 5 \times 5 \times 5\)

\(X^N = X \times X \times X \times ... X\)

\textbf{base}

\textbf{exponenet} (power)


\section{multiplication rule}
\label{sec:org05ea438}

\(x^n \cdot x^m = x^{n+m}\)

\(2^3 \cdot 2^4 = 2^{3 + 4} = 2^7\)

\section{quotient rule}
\label{sec:org7b6b147}

\(\frac{x^n}{x^m} = x^{n - m}\)

\(\frac{3^6}{3^2} = 3^{6 - 2} = 3^4\)

\section{the power rule}
\label{sec:org6676416}

\((x^n)^m = x^{n \cdot m}\)

\((3^2)^3 = (3 \cdot 3) \times (3 \cdot 3) \times (3 \cdot 3)\)

\section{power of zero}
\label{sec:orgea96abb}

\(x^n=0\)

\(x^{n - n} = x^0 = 1\)

\(\frac{2^3}{2^3} = 1\)

\section{negative exponents}
\label{sec:orgedc9c6e}

\(x^{-n} = \frac{1}{x^n}\)

\section{fractional exponents}
\label{sec:org57241cf}

\(x^{\frac{1}{n}} = \sqrt[n]{x}\)

\(64^{\frac{1}{3}} = \sqrt[3]{64}\)

\((5^{\frac{1}{3}})^3 = 5^{\frac{3}{3}} = 5^1 = 5\)

\section{distribute an exponent over a product}
\label{sec:orgd6cf1d2}

\((x \cdot y)^n = x^n \cdot y^n\)

\((5 \cdot 7)^3 = (5 \cdot 7) \times (5 \cdot 7) \times (5 \cdot 7) = 5^3 \cdot 7^3\)

\((\frac{x}{y})^n = \frac{x^n}{y^n}\)

\((\frac{2}{7})^3 = \frac{2}{7} \times \frac{2}{7} \times \frac{2}{7} = \frac{2^3}{7^3}\)

\section{thes apply to only multipilication and division, doesn work with addition and subtraction}
\label{sec:org7694abe}

\((a + b)^n \neq a^n + b^n\)

\$(2 + 3)\textsuperscript{2} \(\neq\) (2\textsuperscript{2} + 3\textsuperscript{2})

\((a - b)^n \neq a^n - b^n\)

\((2 - 3)^2 \neq 2^2 - 3^2\)
\end{document}