#+title:      rational expressions
#+date:       [2023-01-06 Fri 10:21]
#+filetags:   :algebra:math:
#+identifier: 20230106T102143

* rational expresion
- a fraction with variable in it
  \begin{equation*}
  \frac{x + 2}{x^2 - 3}
  \end{equation*}

* simplify to lowest terms
- ex:
  \begin{flalign*}
  \frac{21}{45} &= \frac{7 \cdot 3}{5 \cdot 3 \cdot 3}\\
                &= \frac{7}{15}  
  \end{flalign*}

- ex:
  \begin{flalign*}
  \frac{3x + 6}{x^2 + 4x + 4} &= \frac{3(x + 2)}{(x + 2)(x + 2)}\\
                              &= \frac{3}{x + 2}
  \end{flalign*} 

* Multiplying and Dividing

- ex:
  \begin{flalign*}
  \frac{4}{3} \cdot \frac{2}{5} &= \frac{4 \cdot 2}{3 \cdot 5}\\
                                &= \frac{8}{15}
  \end{flalign*}

- ex:
  \begin{flalign*}
  \frac{\frac{4}{5}}{\frac{2}{3}} &= \frac{4}{3} \cdot \frac{3}{2}\\
                                  &= \frac{12}{10}\\
                                  &= \frac{6}{5} 
  \end{flalign*}

- ex:
  \begin{flalign*}
  \frac{\frac{x^2 + x}{x + 4}}{\frac{x + 1}{x^2 - 16}} &= \frac{x^2 + x}{x + 4} \cdot \frac{x^2 - 16}{x + 1}\\
                                                       &= \frac{(x^2 + x)(x^2 - 16)}{(x + 4)(x + 1)}\\
                                                       &= \frac{x(x + 1)(x + 4)(x - 4)}{(x + 4)(x + 1)}\\
                                                       &= x(x - 4)
  \end{flalign*}

* Adding and Subtracting

- ex:
  - find the LCD: $2 \cdot 3 \cdot 5 = 30$
    
  \begin{flalign*}
  \frac{7}{6} - \frac{4}{15} &= \frac{7}{2 \cdot 3} - \frac{4}{3 \cdot 5}\\
                             &= \frac{35}{30} - \frac{8}{30}\\
                             &= \frac{27}{30}\\
                             &= \frac{3^3}{2 \cdot 3 \cdot 5}\\
                             &= \frac{9}{10}
  \end{flalign*}

- ex:
  \begin{flalign*}
  \frac{3}{2x + 2} + \frac{5}{x^2 - 1} &= \frac{3}{2(x + 1)} + \frac{5}{(x + 1)(x - 1)}\\
                                       &= \frac{3(x - 1)}{2(x + 1)(x - 1)} + \frac{5 \times 2}{2(x + 1)(x - 1)}\\
                                       &= \frac{3(x - 1) + 10}{2(x + 1)(x - 1)}\\
                                       &= \frac{3x + 7}{2(x + 1)(x - 1)}
  \end{flalign*}

* Solving rational expressions
try to get ride of the denomiators by factoring

- ex1:
  \begin{flalign*}
  \frac{x}{x + 3} &= 1 + \frac{1}{x}\\
  ((x + 3)x) \cdot \frac{x}{x + 3} &= (1 + \frac{1}{x}) \cdot ((x + 3)x)\\
  x^2 &= (x + 3)(x) + (x+3)\\
  x^2 &= x^2 + 3x + x + 3\\
  0   &= 4x + 3\\
  4x  &= -3\\
  x   &= -\frac{3}{4}
  \end{flalign*}
  
  - apply LCD: $(x + 3) \cdot x$ to both sides of the equation

- ex2:
  - find LCD of $(c -5),(c + 1)$ and $c^2 - 4c - 5$
    - which is $(c -5),(c + 1)$

  - clear the denominator by factoring
  \begin{flalign*}
  \frac{4c}{c - 5} - \frac{1}{c + 1} &= \frac{3c^2 + 3}{c^2 - 4c - 5}\\
  (c - 5)(c + 1) \cdot \frac{4c}{c - 5}  - (c - 5)(c + 1) \cdot \frac{1}{c + 1} &= (c - 5)(c + 1) \cdot \frac{3c^2 + 3}{(c - 5)(c + 1)}\\ 
  4c^2 + 4c - (c - 5) &= 3c^2 + 3\\
  c^2 + 3c + 5 &= 3\\
  c^2 + 3c + 2 &= 0\\
  (c + 1)(c + 2) &= 0\\
  \end{flalign*}
  
  - c = -1 cause a zero in denominator so cant be the answer

  - c = -2 is the answer.....



